qstar/src/QState.fst
@@ -1,108 +1,68 @@
 module QState
 
 open FStar.Mul
-open FStar.Real
-open Complex
-open Matrix
-open Quantum
+//open FStar.Real
+//open Complex
+//open Matrix
+//open Quantum
 
 module F = FStar.FunctionalExtensionality
 
-// qstate (p,v) = vector v with (classical) probability p
-// TODO: we may want to add the restriction that v has unit norm,
-//       but this will make the definitions below more painful
-type qstate (n:nat) = real & v:matrix complex (pow2 n) 1
-
-// we need to call auxiliary 
-let apply_H #n q qs =
-  let (p,v) = qs in
-  (p, matrix_mul (pad n q hadamard_mat) v)
-
-// similar to apply_H
-let apply_X #n q qs = admit()
-let apply_Z #n q qs = admit()
-let apply_T #n q qs = admit()
-let apply_TDG #n q qs = admit()
-let apply_S #n q qs = admit()
-let apply_SDG #n q qs = admit()
-let apply_CNOT #n q1 q2 qs = admit()
-let apply_CZ #n q1 q2 qs = admit()
-
-let measure #n q r qs = admit()
-  //let (p,v) = qs in
-  //let projv = project q (res_to_bool r) v in
-  //(p *. norm projv, normalize projv)
-
-let init #n qs = 
-  let (p,v) = qs in
-  (p, kronecker_product v (ket false))
-
-let discard #n qs = admit()
-//  let (p,v) = qs in
-//  let projv = matrix_mul (pad n q false) v in
-//  (p *. norm projv, normalize projv)
-
-let classical_state r = admit() //Some (ket (res_to_bool r))
-let plus_state = admit() //Some (F.on (knat 2 & knat 1) (fun (i,j) -> of_real (1.0R /. sqrt_2)))
-let bell00 = admit() //F.on (knat 4 & knat 1) (fun (i,j) -> cmul (of_real (1.0R /. sqrt_2)) (if i = j then c1 else c0))
-
-let extend1 #n q psi = admit()
-let extend2 #n q1 q2 psi = admit()
-
-// check if projecting the current state onto psi leaves the state unchanged
-let in_state #n psi qs =
-  admit() //match qs with
-  //| Some v -> v == (matrix_mul (pad n q (matrix_mul psi (conjugate_transpose psi))) v)
-  //| None -> False
-
-let lemma_apply_H_self_adjoint #n q qs
-  : Lemma (apply_H q (apply_H q qs) == qs)
+let size_disjoint_union (#a:eqtype) (#f:cmp a) (s1 s2:ordset a f)
+  : Lemma (requires (OrdSet.intersect s1 s2 `OrdSet.equal` OrdSet.empty))
+          (ensures (OrdSet.size (union s1 s2) = OrdSet.size s1 + OrdSet.size s2))
+          [SMTPat (size #a #f (union #a #f s1 s2))]
   = admit()
 
-let lemma_apply_X_self_adjoint #n q qs
-  : Lemma (apply_X q (apply_X q qs) == qs)
+let dimension_union (qs0:qbits) (qs1:qbits{disjoint_qbits qs0 qs1})
+  : Lemma (ensures dimension (union qs0 qs1) = dimension qs0 * dimension qs1)
+          [SMTPat (dimension (union qs0 qs1))]
+  = Math.Lemmas.pow2_plus (size qs0) (size qs1)
+
+// Facts about swap matrix (when finished, move to Quantum.fst)
+let swap_mat : matrix complex 4 4 =
+  F.on (knat 4 & knat 4)
+       (fun (i,j) ->
+          if i = 0 && j = 0 then c1
+          else if i = 1 && j = 2 then c1
+          else if i = 2 && j = 1 then c1
+          else if i = 3 && j = 3 then c1
+          else c0)
+
+// can we expose this in the OrdSet interface?
+assume
+val as_list (#a:eqtype) (#f:cmp a) (s:ordset a f) : Tot (l:list a{sorted f l})
+
+// we need some "reorder_indices" function to make the operation commutative
+let tensor #qs0 #qs1 v0 v1 = 
+  admit()
+  //reorder_indices (as_list qs0) (as_list qs1) (kronecker_product v0 v1)
+
+let tensor_unit qs v
+  : Lemma (ensures tensor v empty_qvec == v)
   = admit()
 
-let lemma_apply_Z_self_adjoint #n q qs
-  : Lemma (apply_Z q (apply_Z q qs) == qs)
+let tensor_comm qs0 qs1 v0 v1
+  : Lemma (requires disjoint qs0 qs1)
+          (ensures tensor v0 v1 == tensor v1 v0)
   = admit()
 
-let lemma_apply_T_adjoint #n q qs
-  : Lemma (apply_TDG q (apply_T q qs) == qs)
-  = admit()
+let tensor_assoc_l #qs0 #qs1 #qs2 v0 v1 v2
+   : Lemma (union_ac();
+            tensor (tensor v0 v1) v2 == tensor v0 (tensor v1 v2))
+   = admit()
 
-let lemma_apply_S_adjoint #n q qs
-  : Lemma (apply_SDG q (apply_S q qs) == qs)
-  = admit()
+let tensor_assoc_r #qs0 #qs1 #qs2 v0 v1 v2
+   : Lemma (union_ac ();
+            tensor (tensor v0 v1) v2 == tensor v0 (tensor v1 v2))
+   = admit()
 
-let lemma_apply_CNOT_self_adjoint #n q1 q2 qs
-  : Lemma (apply_CNOT q1 q2 (apply_CNOT q1 q2 qs) == qs)
-  = admit()
-  
-let lemma_apply_CZ_self_adjoint #n q1 q2 qs
-  : Lemma (apply_CZ q1 q2 (apply_CZ q1 q2 qs) == qs)
-  = admit()
+let init #qs v = admit()
 
-let lemma_apply_H_zero #n q qs
-  : Lemma (requires (in_1q_classical_state q Zero qs))
-          (ensures (in_1q_state q plus_state (apply_H q qs)))
-  = admit()
+let disc #qs q v = admit() 
 
-let lemma_apply_H_neq #n q1 q2 psi qs
-  : Lemma (requires (in_1q_state q2 psi qs))
-          (ensures (in_1q_state q2 psi (apply_H q1 qs)))
-  = admit()
+let meas #qs q b v = admit() 
 
-let lemma_apply_CNOT_plus #n q1 q2 qs
-  : Lemma (requires (in_1q_state q1 plus_state qs /\ in_1q_classical_state q2 Zero qs))
-          (ensures (in_2q_state q1 q2 bell00 (apply_CNOT q1 q2 qs)))
-  = admit()
+let applyH #qs q v = admit() 
 
-let lemma_meas_result #n q r qs
-  : Lemma (ensures (in_1q_classical_state q r (snd (measure q r qs))))
-  = admit()
-
-let lemma_pauli_x #n q r qs
-  : Lemma (requires (in_1q_classical_state q r qs))
-          (ensures (in_1q_classical_state q (neg_res r) (apply_X q qs)))
-  = admit()
+let applyCX #qs q1 q2 v = admit() 
