qstar/src/QState.fsti
@@ -1,119 +1,110 @@
 module QState
-open FStar.Real
+
+open Complex
+open Matrix
+open FStar.Seq
+open FStar.OrdSet
 
 (* This module defines our representation of quantum states, operations 
    acting on quantum states, and predicates for describing quantum
-   states. 
-   
-   We leave everything abstract in the interface file to allow for
-   different implementation choices down the road. *)
+   states. *)
 
-// type for a quantum state
-val qstate (n:nat) : Type0
+let qbit = nat
 
-// type for an index into the quantum state
-type qloc (k:nat) = n:nat{n < k}
+let qbits = OrdSet.ordset qbit (<=)
 
-// measurement outcome type
-type result = | Zero | One
-let res_to_bool r = match r with Zero -> false | One -> true
-let bool_to_res b = if b then One else Zero
+let dimension (qs:qbits) = pow2 (OrdSet.size qs)
 
-let neg_res r = match r with Zero -> One | One -> Zero
+// TODO: add restriction of unit norm?
+let qvec (qs:qbits) = matrix complex (dimension qs) 1
 
-let xor_res r1 r2 = 
-  match r1, r2 with 
-  | Zero, Zero | One, One -> Zero 
-  | _, _ -> One
+let empty_qbits : qbits = OrdSet.empty
 
-let and_res r1 r2 = 
-  match r1, r2 with 
-  | One, One -> One
-  | _, _ -> Zero
+let empty_qvec : qvec empty_qbits = id_matrix complex 1
 
-// apply a gate
-val apply_H : (#n:nat) -> qloc n -> qstate n -> qstate n
-val apply_X : (#n:nat) -> qloc n -> qstate n -> qstate n
-val apply_Z : (#n:nat) -> qloc n -> qstate n -> qstate n
-val apply_T : (#n:nat) -> qloc n -> qstate n -> qstate n
-val apply_TDG : (#n:nat) -> qloc n -> qstate n -> qstate n
-val apply_S : (#n:nat) -> qloc n -> qstate n -> qstate n
-val apply_SDG : (#n:nat) -> qloc n -> qstate n -> qstate n
-val apply_CNOT : (#n:nat) -> (q1:qloc n) -> (q2:qloc n{q1 <> q2}) -> qstate n -> qstate n
-val apply_CZ : (#n:nat) -> (q1:qloc n) -> (q2:qloc n{q1 <> q2}) -> qstate n -> qstate n
+let disjoint_qbits (q0 q1:qbits) = (OrdSet.intersect q0 q1 `OrdSet.equal` empty_qbits)
 
-// project a quantum state onto a given measurement outcome, returning
-// the probability of that outcome and the resulting state
-val measure : (#n:nat) -> qloc n -> result -> qstate n -> real & qstate n
+let union_empty (q:qbits)
+  : Lemma (union q empty_qbits `OrdSet.equal` q)
+          [SMTPat (union q empty_qbits)]
+  = ()
 
-// extend the state with a fresh |0> qubit
-val init : (#n:nat) -> qstate n -> qstate (n+1)
+let union_ac ()
+  : Lemma ((forall (qs0 qs1 qs2:qbits).
+              union qs0 (union qs1 qs2) `OrdSet.equal` union (union qs0 qs1) qs2) /\
+           (forall (qs0 qs1:qbits).
+              union qs0 qs1 `OrdSet.equal` union qs1 qs0) /\
+           (forall (q:qbits). union q empty_qbits `OrdSet.equal` q))
+  = ()
 
-// discard the last qubit
-val discard : (#n:nat{n > 0}) -> qstate n -> qstate (n-1)
+val tensor (#qs0:qbits)
+           (#qs1:qbits {disjoint_qbits qs0 qs1})
+           (v0:qvec qs0)
+           (v1:qvec qs1)
+  : qvec (union qs0 qs1)
 
-// some common states
-val classical_state : result -> qstate 1 // |0> or |1>
-val plus_state : qstate 1 // |+> = 1/sqrt(2) * (|0> + |1>)
-val bell00 : qstate 2 // 1 / sqrt(2) * (|00> + |11>)
+val tensor_unit (qs:qbits) (v:qvec qs)
+  : Lemma
+    (ensures tensor v empty_qvec == v)
 
-// extend a 1- or 2-qubit state to the full n dimensions
-val extend1 : (#n:nat{n>=1}) -> qloc n -> qstate 1 -> qstate n
-val extend2 : (#n:nat{n>=2}) -> q1:qloc n -> q2:qloc n{q1 <> q2} -> qstate 2 -> qstate n
+val tensor_comm (qs0 qs1:qbits) (v0:qvec qs0) (v1:qvec qs1)
+  : Lemma
+    (requires disjoint qs0 qs1)
+    (ensures tensor v0 v1 == tensor v1 v0)
 
-// "in_state qs1 qs2" says that state qs2 is in state qs1
-val in_state : (#n:nat) -> qstate n -> qstate n -> prop
-let in_1q_state (#n:nat{n>=1}) (q:qloc n) (qs:qstate 1) (qs':qstate n) =
-  in_state (extend1 q qs) qs'
-let in_1q_classical_state (#n:nat{n>=1}) (q:qloc n) (r:result) (qs:qstate n) =
-  in_1q_state q (classical_state r) qs
-let in_2q_state (#n:nat{n>=2}) (q1:qloc n) (q2:qloc n{q1 <> q2}) (qs:qstate 2) (qs':qstate n) =
-  in_state (extend2 q1 q2 qs) qs'
+val tensor_assoc_l (#qs0:_)
+                   (#qs1:_{disjoint_qbits qs0 qs1})
+                   (#qs2:_{disjoint_qbits (OrdSet.union qs0 qs1) qs2})
+                   (v0:qvec qs0)
+                   (v1:qvec qs1)
+                   (v2:qvec qs2)
+   : Lemma (union_ac();
+            tensor (tensor v0 v1) v2 == tensor v0 (tensor v1 v2))
 
-val lemma_apply_H_self_adjoint (#n:nat) (q:qloc n) (qs:qstate n)
-  : Lemma (apply_H q (apply_H q qs) == qs)
-    [SMTPat (apply_H q (apply_H q qs))]
+val tensor_assoc_r (#qs0:_)
+                   (#qs1:_)
+                   (#qs2:_{disjoint_qbits qs1 qs2 /\ disjoint_qbits qs0 (OrdSet.union qs1 qs2)})
+                   (v0:qvec qs0)
+                   (v1:qvec qs1)
+                   (v2:qvec qs2)
+   : Lemma (union_ac ();
+            tensor (tensor v0 v1) v2 == tensor v0 (tensor v1 v2))
 
-val lemma_apply_X_self_adjoint (#n:nat) (q:qloc n) (qs:qstate n)
-  : Lemma (apply_X q (apply_X q qs) == qs)
-    [SMTPat (apply_X q (apply_X q qs))]
+// operations:
+// * init
+// * disc
+// * apply
+// * meas
 
-val lemma_apply_Z_self_adjoint (#n:nat) (q:qloc n) (qs:qstate n)
-  : Lemma (apply_Z q (apply_Z q qs) == qs)
-    [SMTPat (apply_Z q (apply_Z q qs))]
+val init : (#qs:qbits) -> qvec qs -> (q:qbit) & qvec (union qs (singleton q))
 
-val lemma_apply_T_adjoint (#n:nat) (q:qloc n) (qs:qstate n)
-  : Lemma (apply_TDG q (apply_T q qs) == qs)
-    [SMTPat (apply_TDG q (apply_T q qs))]
+val disc : (#qs:qbits) -> (q:qbit{mem q qs}) -> qvec qs -> qvec (remove q qs) 
 
-val lemma_apply_S_adjoint (#n:nat) (q:qloc n) (qs:qstate n)
-  : Lemma (apply_SDG q (apply_S q qs) == qs)
-    [SMTPat (apply_SDG q (apply_S q qs))]
+val meas : (#qs:qbits) -> (q:qbit{mem q qs}) -> bool -> qvec qs -> qvec qs
 
-val lemma_apply_CNOT_self_adjoint (#n:nat) (q1:qloc n) (q2:qloc n{q1 <> q2}) (qs:qstate n)
-  : Lemma (apply_CNOT q1 q2 (apply_CNOT q1 q2 qs) == qs)
-    [SMTPat (apply_CNOT q1 q2 (apply_CNOT q1 q2 qs))]
+val applyH : (#qs:qbits) -> (q:qbit{mem q qs}) -> qvec qs -> qvec qs
 
-val lemma_apply_CZ_self_adjoint (#n:nat) (q1:qloc n) (q2:qloc n{q1 <> q2}) (qs:qstate n)
-  : Lemma (apply_CZ q1 q2 (apply_CZ q1 q2 qs) == qs)
-    [SMTPat (apply_CZ q1 q2 (apply_CZ q1 q2 qs))]
+val applyCX : (#qs:qbits) -> (q1:qbit{mem q1 qs}) -> 
+              (q2:qbit{mem q2 qs /\ q1 <> q2}) -> qvec qs -> qvec qs
 
-// axiomatic-style specs for gates
-val lemma_apply_H_zero (#n:nat) (q:qloc n) (qs:qstate n)
-  : Lemma (requires (in_1q_classical_state q Zero qs))
-          (ensures (in_1q_state q plus_state (apply_H q qs)))
+// The pts_to predicate says that a set of qubits is in a particular vector state v
 
-val lemma_apply_H_neq (#n:nat) (q1:qloc n) (q2:qloc n{q1 <> q2}) (psi:qstate 1) (qs:qstate n)
-  : Lemma (requires (in_1q_state q2 psi qs))
-          (ensures (in_1q_state q2 psi (apply_H q1 qs)))
+(* From Nik:
 
-val lemma_apply_CNOT_plus (#n:nat) (q1:qloc n) (q2:qloc n{q1 <> q2}) (qs:qstate n)
-  : Lemma (requires (in_1q_state q1 plus_state qs /\ in_1q_classical_state q2 Zero qs))
-          (ensures (in_2q_state q1 q2 bell00 (apply_CNOT q1 q2 qs)))
+When implementing a frame-preserving update for an action (e.g., like applying a gate to some qs), we get to assume that whatever precondition P that the caller provides is compatible with the current full heap H0. And we have to update the full heap to H1, returning the postcondition Q, and proving that whatever other frame F was composable with P and compatible with H0, is now also composable with Q and compatible with H1.
+*)
 
-val lemma_meas_result (#n:nat) (q:qloc n) (r:result) (qs:qstate n)
-  : Lemma (ensures (in_1q_classical_state q r (snd (measure q r qs))))
+(* From FStar.PCM:
 
-val lemma_pauli_x (#n:nat) (q:qloc n) (r:result) (qs:qstate n)
-  : Lemma (requires (in_1q_classical_state q r qs))
-          (ensures (in_1q_classical_state q (neg_res r) (apply_X q qs)))
+type frame_preserving_upd (#a:Type u#a) (p:pcm a) (x y:a) =
+  v:a{
+    p.refine v /\
+    compatible p x v
+  } ->
+  v_new:a{
+    p.refine v_new /\
+    compatible p y v_new /\
+    (forall (frame:a{composable p x frame}).{:pattern composable p x frame}
+       composable p y frame /\
+       (op p x frame == v ==> op p y frame == v_new))}
+*)
