qstar/src/QStarHeap.fst
@@ -1,0 +1,114 @@
+module QStarHeap
+open FStar.PCM
+open FStar.OrdSet
+open FStar.Real
+module Frac = Steel.FractionalPermission
+
+open QState
+
+noeq
+type qstate = {
+  frac:option Frac.perm;
+  qs:qbits;
+  state:qvec qs;
+}
+
+let unit_qstate = { frac=None; qs=empty_qbits; state=empty_qvec}
+
+let composable_frac_opt (f0 f1:option Frac.perm)
+  : Type
+  = match f0, f1 with
+    | None, _
+    | _, None -> True
+    | Some p0, Some p1 ->
+      Frac.(sum_perm p0 p1 `lesser_equal_perm` full_perm)
+
+let compose_frac_opt (f0:option Frac.perm)
+                     (f1:option Frac.perm { composable_frac_opt f0 f1 })
+  : option Frac.perm
+  = match f0, f1 with
+    | None, f
+    | f, None -> f
+    | Some f0, Some f1 -> Some (Frac.sum_perm f0 f1)
+
+let composable
+  : symrel qstate
+  = fun (q0 q1:qstate) ->
+      composable_frac_opt q0.frac q1.frac /\
+      disjoint_qbits q0.qs q1.qs
+
+let compose (q0:qstate) (q1:qstate{composable q0 q1})
+  : qstate
+  = { frac = compose_frac_opt q0.frac q1.frac;
+      qs = OrdSet.union q0.qs q1.qs;
+      state = q0.state `tensor` q1.state }
+
+let core : pcm' qstate = {
+  composable;
+  op = compose;
+  one = unit_qstate
+}
+
+#push-options "--fuel 0 --ifuel 1 --z3rlimit_factor 3"
+let tensor_ac ()
+  : Lemma (union_ac();
+           // tensor is a PCM
+           (forall (qs0:_) (qs1:_{disjoint_qbits qs0 qs1}) (v0:qvec qs0) (v1:qvec qs1).
+              tensor v0 v1 == tensor v1 v0) /\
+           (forall (qs0:_)
+              (qs1:_{disjoint_qbits qs0 qs1})
+              (qs2:_{disjoint_qbits (OrdSet.union qs0 qs1) qs2})
+              (v0:qvec qs0)
+              (v1:qvec qs1)
+              (v2:qvec qs2).
+              tensor (tensor v0 v1) v2 == tensor v0 (tensor v1 v2)) /\
+           (forall (qs0:_)
+              (qs1:_)
+              (qs2:_{disjoint_qbits qs1 qs2 /\ disjoint_qbits qs0 (OrdSet.union qs1 qs2)})
+              (v0:qvec qs0)
+              (v1:qvec qs1)
+              (v2:qvec qs2).
+              tensor (tensor v0 v1) v2 == tensor v0 (tensor v1 v2)) /\
+           (forall qs0 (v0:qvec qs0).
+              tensor v0 empty_qvec == v0))
+  = union_ac();
+    introduce forall (qs0:_) (qs1:_{disjoint_qbits qs0 qs1}) (v0:qvec qs0) (v1:qvec qs1).
+              tensor v0 v1 == tensor v1 v0
+    with tensor_comm qs0 qs1 v0 v1;
+
+    introduce forall qs0 (v0:qvec qs0). tensor v0 empty_qvec == v0
+    with tensor_unit _ v0;
+
+    introduce forall (qs0:_)
+                (qs1:_{disjoint_qbits qs0 qs1})
+                (qs2:_{disjoint_qbits (OrdSet.union qs0 qs1) qs2})
+                (v0:qvec qs0)
+                (v1:qvec qs1)
+                (v2:qvec qs2).
+              tensor (tensor v0 v1) v2 == tensor v0 (tensor v1 v2)
+    with tensor_assoc_l v0 v1 v2;
+
+    introduce forall (qs0:_)
+                (qs1:_)
+                (qs2:_{disjoint_qbits qs1 qs2 /\ disjoint_qbits qs0 (OrdSet.union qs1 qs2)})
+                (v0:qvec qs0)
+                (v1:qvec qs1)
+                (v2:qvec qs2).
+              tensor (tensor v0 v1) v2 == tensor v0 (tensor v1 v2)
+    with tensor_assoc_r v0 v1 v2
+#pop-options
+
+// a bit lazy: just calling tensor AC and letting the SMT solver do the rest
+#push-options "--fuel 0 --ifuel 1 --z3rlimit_factor 3"
+let qstar_heap_pcm : pcm qstate =
+  union_ac();
+  tensor_ac ();
+{
+  p = core;
+  comm = (fun _ _ -> ());
+  assoc = (fun _ _ _ -> ());
+  assoc_r = (fun _ _ _ -> ());
+  is_unit = (fun _ -> ());
+  refine = (fun qs -> qs.frac == Some Frac.full_perm)
+}
+#pop-options
